BVP simp opt improved: right assoc Seq

new-backend/bvp_simpScript.sml
@@ -5,8 +5,6 @@ open finite_mapTheory sumTheory relationTheory stringTheory optionTheory;
 open bytecodeTheory bvlTheory bvpTheory;
 open sptreeTheory lcsymtacs;
 
-infix \\ val op \\ = op THEN;
-
 (* Simple clean up of BVP:
 
    The pSimp optimisation removes Skips and deteles some dead code
@@ -14,9 +12,13 @@ infix \\ val op \\ = op THEN;
 
      Seq (Seq Skip (Raise n)) anything_here
 
-   translates into:
+   translates into
 
      Raise n
+
+   It also right-associates Seq, e.g.
+
+     Seq (Seq x1 x2) x3 --> Seq x1 (Seq x2 x3)
 
 *)
 
@@ -26,60 +28,47 @@ val isSkip_def = Define `
 
 val pSeq_def = Define `
   pSeq c1 c2 =
-    if isSkip c1 then c2 else
     if isSkip c2 then c1 else Seq c1 c2`;
 
 val pSimp_def = Define `
-  (pSimp (Return n) = (Return n,T)) /\
-  (pSimp (Raise n) = (Raise n,T)) /\
-  (pSimp (Seq c1 c2) =
-        let (d1,r1) = pSimp c1 in
-        let (d2,r2) = pSimp c2 in
-          if r1 then (d1,r1) else (pSeq d1 d2,r2)) /\
-  (pSimp (Handle c1 n1 n2 c2) =
-     (Handle (FST (pSimp c1)) n1 n2 (FST (pSimp c2)),F)) /\
-  (pSimp (If c1 n c2 c3) =
-        let (d1,r1) = pSimp c1 in
-        let (d2,r2) = pSimp c2 in
-        let (d3,r3) = pSimp c3 in
-          if r1 then (d1,r1) else
-            (If d1 n d2 d3,r2 /\ r3)) /\
-  (pSimp c = (c,F))`;
+  (pSimp Skip c = c) /\
+  (pSimp (Return n) c = Return n) /\
+  (pSimp (Raise n) c = Raise n) /\
+  (pSimp (Seq c1 c2) c = pSimp c1 (pSimp c2 c)) /\
+  (pSimp (Handle c1 n1 n2 c2) c =
+     pSeq (Handle (pSimp c1 Skip) n1 n2 (pSimp c2 Skip)) c) /\
+  (pSimp (If c1 n c2 c3) c =
+     pSeq (If (pSimp c1 Skip) n (pSimp c2 Skip) (pSimp c3 Skip)) c) /\
+  (pSimp c1 c2 = pSeq c1 c2)`;
 
 val isSkip_thm = prove(
   ``!c. isSkip c = (c = Skip)``,
   Cases \\ SRW_TAC [] [isSkip_def]);
 
+val pEval_Seq_Skip = prove(
+  ``!c s. pEval (Seq c Skip,s) = pEval (c,s)``,
+  fs [pEval_def,LET_DEF] \\ REPEAT STRIP_TAC
+  \\ Cases_on `pEval (c,s)` \\ fs [] \\ SRW_TAC [] []);
+
 val pEval_pSeq = prove(
   ``pEval (pSeq c1 c2, s) = pEval (Seq c1 c2, s)``,
-  SRW_TAC [] [pSeq_def] \\ fs [isSkip_thm]
-  \\ SIMP_TAC std_ss [pEval_def,LET_DEF]
-  \\ Cases_on `pEval (c1,s)` \\ fs [] \\ SRW_TAC [] []);
-
-val FST_LEMMA = prove(
-  ``!foo. (foo = (x1,x2)) ==> (FST foo = x1)``,
-  Cases \\ SRW_TAC [] []);
-
-val lemma = METIS_PROVE [] ``(!x. P x /\ Q x) <=> (!x. P x) /\ (!x. Q x)``;
+  SRW_TAC [] [pSeq_def] \\ fs [isSkip_thm,pEval_Seq_Skip]);
 
 val pEval_pSimp = prove(
-  ``(!c s. (pEval (FST (pSimp c),s) = pEval (c,s)) /\
-           (SND (pSimp c) ==> (FST (pEval (c,s)) <> NONE)))``,
-  HO_MATCH_MP_TAC (fetch "-" "pSimp_ind") \\ REPEAT STRIP_TAC
-  \\ FULL_SIMP_TAC (srw_ss()) [pSimp_def,pEval_def,pEval_pSeq]
-  \\ REPEAT BasicProvers.FULL_CASE_TAC \\ fs []
-  \\ SRW_TAC [] [pEval_pSeq,pEval_def]
-  \\ fs [] \\ SRW_TAC [] [] \\ fs [pEval_pSeq,pEval_def,LET_DEF]
-  \\ Cases_on `pSimp c` \\ fs []
-  \\ Cases_on `pSimp c'` \\ fs []
-  \\ Cases_on `pSimp c''` \\ fs [] \\ SRW_TAC [] []
-  \\ Cases_on `pEval (c,s)` \\ fs []
-  \\ REPEAT BasicProvers.FULL_CASE_TAC \\ SRW_TAC [] [] \\ fs [lemma]
-  \\ IMP_RES_TAC FST_LEMMA \\ fs []
-  \\ METIS_TAC [optionTheory.NOT_SOME_NONE,FST]);
+  ``!c1 s c2. pEval (pSimp c1 c2,s) = pEval (Seq c1 c2,s)``,
+  recInduct pEval_ind \\ REPEAT STRIP_TAC
+  \\ fs [pSimp_def,pEval_def,LET_DEF,pEval_pSeq,pEval_pSeq]
+  \\ Cases_on `pEval (c1,s)` \\ fs []
+  \\ Cases_on `pEval (c2,r)` \\ fs []
+  \\ Cases_on `pEval (c2,set_var n b r)` \\ fs []
+  \\ Cases_on `pEval (g,s)` \\ fs []
+  \\ REPEAT (BasicProvers.FULL_CASE_TAC \\ fs [pEval_def])
+  \\ fs [EVAL ``bool_to_val F = bool_to_val T``]
+  \\ CONV_TAC (DEPTH_CONV (PairRules.PBETA_CONV))
+  \\ REPEAT (BasicProvers.FULL_CASE_TAC \\ fs [pEval_def]));
 
 val pSimp_thm = store_thm("pSimp_thm",
-  ``!c s. pEval (FST (pSimp c),s) = pEval (c,s)``,
-  fs [pEval_pSimp]);
+  ``!c s. pEval (pSimp c Skip,s) = pEval (c,s)``,
+  SIMP_TAC std_ss [pEval_pSimp,pEval_Seq_Skip]);
 
 val _ = export_theory();
